coq:STLC

coq/Logic/STLC/Replace.v
@@ -2,23 +2,23 @@ Require Import Logic.Class.Eq.
 
 Require Import Logic.STLC.Syntax.
 
-Definition replace (b v:Type) (e:Eq v) (x:v) (t:Exp b v) (u:v) : Exp b v :=
+Definition replace (b v:Type) (eq:Eq v) (x:v) (e:Exp b v) (u:v) : Exp b v :=
     match eqDec u x with
-    | left _    => t
+    | left _    => e
     | right _   => Var u
     end.
 
-Arguments replace {b} {v} {e}.
+Arguments replace {b} {v} {eq}.
 
-Notation "t // x" := (replace x t)
+Notation "e // x" := (replace x e)
     (at level 70, no associativity) : STLC_Replace_scope.
 
 Open Scope STLC_Replace_scope.
 
-Lemma replace_x : forall (b v:Type) (e:Eq v) (x:v) (t:Exp b v),
-    (t // x) x = t.
+Lemma replace_x : forall (b v:Type) (eq:Eq v) (x:v) (e:Exp b v),
+    (e // x) x = e.
 Proof.
-    intros b v e x t. unfold replace. destruct (eqDec x x) as [H1|H1].
+    intros b v eq x e. unfold replace. destruct (eqDec x x) as [H1|H1].
     - reflexivity.
     - exfalso. apply H1. reflexivity.
 Qed.
