coq/Logic/STLC/Subst.v
@@ -5,33 +5,33 @@ Require Import Logic.Class.Eq.
 
 Require Import Logic.STLC.Syntax.
 
-Fixpoint subst_(b v:Type)(e:Eq v)(f:v -> Exp b v)(xs:list v)(t:Exp b v):Exp b v:=
-    match t with
-    | Ann t' Ty => Ann (subst_ b v e f xs t') Ty
+Fixpoint subst_(b v:Type)(eq:Eq v)(f:v -> Exp b v)(xs:list v)(e:Exp b v):Exp b v:=
+    match e with
+    | Ann e' Ty => Ann (subst_ b v eq f xs e') Ty
     | Var x     =>
         match in_dec eqDec x xs with
         | left _    => Var x    (* x is deemed bound    -> Var x                *)
         | right _   => f x      (* x is deemed free     -> f x                  *)
         end
-    | App t1 t2 => App (subst_ b v e f xs t1) (subst_ b v e f xs t2)
-    | Lam x t1  => Lam x (subst_ b v e f (x :: xs) t1)  (* x now bound          *)
+    | App t1 t2 => App (subst_ b v eq f xs t1) (subst_ b v eq f xs t2)
+    | Lam x t1  => Lam x (subst_ b v eq f (x :: xs) t1)  (* x now bound         *)
     end.
-Arguments subst_ {b} {v} {e}.
+Arguments subst_ {b} {v} {eq}.
 
-Definition subst(b v:Type)(e:Eq v)(f:v -> Exp b v)(t:Exp b v):Exp b v:=
-    subst_ f [] t.
+Definition subst(b v:Type)(eq:Eq v)(f:v -> Exp b v)(e:Exp b v):Exp b v:=
+    subst_ f [] e.
 
-Arguments subst {b} {v} {e}.
+Arguments subst {b} {v} {eq}.
 
-Lemma substAnn : forall (b v:Type)(e:Eq v)(f:v -> Exp b v)(t:Exp b v)(Ty:T b),
-    subst f (Ann t Ty) = Ann (subst f t) Ty.
-Proof. intros b v e f t Ty. reflexivity. Qed.
+Lemma substAnn : forall (b v:Type)(eq:Eq v)(f:v -> Exp b v)(e:Exp b v)(Ty:T b),
+    subst f (Ann e Ty) = Ann (subst f e) Ty.
+Proof. intros b v eq f e Ty. reflexivity. Qed.
 
-Lemma substVar : forall (b v:Type)(e:Eq v)(f:v -> Exp b v)(x:v),
+Lemma substVar : forall (b v:Type)(eq:Eq v)(f:v -> Exp b v)(x:v),
     subst f (Var x) = f x.
-Proof. intros b v e f x. reflexivity. Qed.
+Proof. intros b v eq f x. reflexivity. Qed.
 
-Lemma substApp : forall (b v:Type)(e:Eq v)(f:v -> Exp b v)(t1 t2:Exp b v),
-    subst f (App t1 t2) = App (subst f t1) (subst f t2).
-Proof. intros b v e f t1 t2. reflexivity. Qed.
+Lemma substApp : forall (b v:Type)(eq:Eq v)(f:v -> Exp b v)(e1 e2:Exp b v),
+    subst f (App e1 e2) = App (subst f e1) (subst f e2).
+Proof. intros b v eq f e1 e2. reflexivity. Qed.
 
