coq/Logic/STLC/Valid.v
@@ -4,8 +4,8 @@ Require Import Logic.STLC.Context.
 
 Inductive Valid (b v:Type) : @Context b v -> Prop :=
 | ValidO   : Valid b v O
-| ValidTy  : forall (G:Context) (Ty:b),
-    Valid b v G -> Valid b v (G ; Ty ::: *)
+| ValidTy  : forall (G:Context) (t:b),
+    Valid b v G -> Valid b v (G ; t ::: *)
 | ValidVar : forall (G:Context) (x:v) (Ty:T b),
     Valid b v G -> G :- Ty -> Valid b v (G ; x ::: Ty) 
 .
@@ -16,18 +16,18 @@ Arguments ValidTy  {b} {v}.
 Arguments ValidVar {b} {v}.
 
 (* An example of valid context                                                  *)
-Definition G1 (base v:Type) (a b:base) (const:v) : @Context base v 
+Definition G1 (b v:Type) (t t':b) (const:v) : @Context b v 
     := O
-    ; a ::: *
-    ; b ::: *
-    ; const ::: ((Base b :-> Base b) :-> Base a :-> Base b :-> Base b)
+    ; t  ::: *
+    ; t' ::: *
+    ; const ::: ((Base t' :-> Base t') :-> Base t :-> Base t' :-> Base t')
     .
-Arguments G1 {base} {v}.
+Arguments G1 {b} {v}.
 
-Lemma ValidG1 : forall (base v:Type) (a b:base) (const:v),
-    Valid (G1 a b const).
+Lemma ValidG1 : forall (b v:Type) (t t':b) (const:v),
+    Valid (G1 t t' const).
 Proof.
-    intros base v a b const. constructor.
+    intros b v t t' const. constructor.
     - constructor. constructor. constructor.
     - constructor.
         + constructor; constructor; apply FindTyZ.
