coq/Logic/STLC/Context.v
@@ -33,49 +33,46 @@ Notation "G ; x" := (CtxSnoc G x)
 Open Scope STLC_Context_scope.
 
 Inductive FindTy (b v:Type) : @Context b v -> b -> Prop :=
-| FindTyZ : forall (G:Context) (Ty:b), FindTy b v (G ; Ty ::: *) Ty
-| FindTyS : forall (G:Context) (Ty:b) (k:Binding),
-    FindTy b v G Ty -> FindTy b v (G ; k) Ty
+| FindTyZ : forall (G:Context) (t:b), FindTy b v (G ; t ::: *) t
+| FindTyS : forall (G:Context) (t:b) (k:Binding),
+    FindTy b v G t -> FindTy b v (G ; k) t
 .
 
 Arguments FindTy  {b} {v}.
 Arguments FindTyZ {b} {v}.
 Arguments FindTyS {b} {v}.
 
-
-
 Notation "G :> Ty" := (FindTy G Ty)
     (at level 60, no associativity) : STLC_Context_scope.
 
-Lemma findTyRev : forall (b v:Type) (G:Context) (x:v) (Sy:T b) (Ty : b),
-    G ; x ::: Sy :> Ty -> G :> Ty.
+Lemma findTyRev : forall (b v:Type) (G:Context) (x:v) (Ty:T b) (t : b),
+    G ; x ::: Ty :> t -> G :> t.
 Proof.
-    intros b v G x Sy Ty H1. remember (G ; x ::: Sy) as G' eqn:E.
-    revert G x Sy E. destruct H1 as [G Ty|G Ty k H1]; intros G' x Sy H2.
+    intros b v G x Ty t H1. remember (G ; x ::: Ty) as G' eqn:E.
+    revert G x Ty E. destruct H1 as [G t|G t k H1]; intros G' x Ty H2.
     - inversion H2. 
     - inversion H2. subst. assumption.
 Qed.
 
-Lemma findTyRev' : forall (b v:Type) (G:@Context b v) (Ty Ty':b),
-    G ; Ty ::: * :> Ty' -> Ty = Ty' \/ G :> Ty'.
+Lemma findTyRev' : forall (b v:Type) (G:@Context b v) (t t':b),
+    G ; t ::: * :> t' -> t = t' \/ G :> t'.
 Proof.
-    intros b v G Ty Ty' H1. remember (G;Ty ::: *) as G' eqn:E.
-    revert G Ty E. destruct H1 as [G Ty|G Ty k H2];
-    intros G' Ty' H3; inversion H3. 
+    intros b v G t t' H1. remember (G;t ::: *) as G' eqn:E.
+    revert G t E. destruct H1 as [G t|G t k H2];
+    intros G' t' H3; inversion H3. 
     - left. reflexivity.
     - subst. right. assumption.
 Qed.
 
-
 Inductive FindVar (b v:Type) (e:Eq v) : @Context b v -> @Binding b v -> Prop :=
 | FindVarZ : forall (G:Context) (x:v) (Ty:T b), 
     FindVar b v e (G ; x ::: Ty) (x ::: Ty)
-| FindVarSkip : forall (G:Context) (k:Binding) (Ty:b),
-    FindVar b v e G k -> FindVar b v e (G ; Ty ::: * ) k
-| FindVarS : forall (G:Context) (x y:v) (Ty Sy:T b),
-    x <> y                                  ->
-    FindVar b v e G (x ::: Ty)              ->
-    FindVar b v e (G ; y ::: Sy) (x ::: Ty)
+| FindVarSkip : forall (G:Context) (k:Binding) (t:b),
+    FindVar b v e G k -> FindVar b v e (G ; t ::: * ) k
+| FindVarS : forall (G:Context) (x y:v) (Ty Ty':T b),
+    x <> y                                      ->
+    FindVar b v e G (x ::: Ty)                  ->
+    FindVar b v e (G ; y ::: Ty') (x ::: Ty)
 .
 
 Arguments FindVar     {b} {v} {e}.
@@ -86,20 +83,20 @@ Arguments FindVarS    {b} {v} {e}.
 Notation "G :>> k" := (FindVar G k)
     (at level 60, no associativity) : STLC_Context_scope.
 
-Lemma findVarRev : forall (b v:Type) (e:Eq v) (G:Context) (Sy:b) (x:v) (Ty:T b),
-    G ; Sy ::: * :>> x ::: Ty -> G :>> x ::: Ty.
+Lemma findVarRev : forall (b v:Type) (e:Eq v) (G:Context) (t:b) (x:v) (Ty:T b),
+    G ; t ::: * :>> x ::: Ty -> G :>> x ::: Ty.
 Proof.
-    intros b v e G Sy x Ty H1.
-    remember (G ; Sy ::: *) as G' eqn:E. remember (x ::: Ty) as k eqn:F.
-    revert G Sy x Ty E F. destruct H1 as [G x Ty|G k Ty H1|G x y Ty Uy H1 H2];
-    intros G' Sy x' Ty' H3 H4. 
+    intros b v e G t x Ty H1.
+    remember (G ; t ::: *) as G' eqn:E. remember (x ::: Ty) as k eqn:F.
+    revert G t x Ty E F. destruct H1 as [G x Ty|G k Ty H1|G x y Ty Ty' H1 H2];
+    intros G' t x' Sy H3 H4. 
     - inversion H3.
     - inversion H3. subst. assumption.
     - inversion H3.
 Qed.
 
 Definition ctxIncl (b v:Type)(e:Eq v)(G H:@Context b v) : Prop :=
-    (forall (Ty:b), G :> Ty -> H :> Ty) /\
+    (forall (t:b), G :> t -> H :> t) /\
     (forall (x:v) (Ty:T b), G :>> x ::: Ty -> H :>> x ::: Ty).
 
 Arguments ctxIncl {b} {v} {e}.
@@ -129,16 +126,16 @@ Lemma ctxInclTrans : forall (b v:Type) (e:Eq v) (G H K:@Context b v),
     G <= H -> H <= K -> G <= K.
 Proof. intros b v e G H K [H1 H2] [H3 H4]. split; auto. Qed.
 
-Lemma ctxInclExtendTy : forall (b v:Type) (e:Eq v) (G H:@Context b v) (Ty:b),
-    G <= H -> G ; Ty ::: * <= H ; Ty ::: *.
+Lemma ctxInclExtendTy : forall (b v:Type) (e:Eq v) (G H:@Context b v) (t:b),
+    G <= H -> G ; t ::: * <= H ; t ::: *.
 Proof.
-    intros b v e G H Ty [H1 H2]. split.
-    - intros Ty' H3.  remember (G ; Ty ::: * ) as G' eqn:E.
-      revert G H H1 H2 Ty E. destruct H3 as [G Ty|G Ty k H1].
-        + intros G' H H2 H3 Ty' H4. inversion H4. apply FindTyZ.
-        + intros G' H H2 H3 Ty' H4. inversion H4. subst.
+    intros b v e G H t [H1 H2]. split.
+    - intros t' H3.  remember (G ; t ::: * ) as G' eqn:E.
+      revert G H H1 H2 t E. destruct H3 as [G t|G t k H1].
+        + intros G' H H2 H3 t' H4. inversion H4. apply FindTyZ.
+        + intros G' H H2 H3 t' H4. inversion H4. subst.
           apply FindTyS, H2. assumption.
-    - intros x Ty' H3. constructor. apply H2. apply findVarRev in H3. assumption.
+    - intros x t' H3. constructor. apply H2. apply findVarRev in H3. assumption.
 Qed.
 
 Lemma ctxInclExtendVar : forall (b v:Type)(e:Eq v)(G H:@Context b v)(x:v)(Ty:T b),
@@ -156,4 +153,3 @@ Proof.
         + inversion H5. subst. apply FindVarS; try assumption. 
           apply H4. assumption.
 Qed.
-
