coq/Logic/STLC/Eval.v
@@ -11,37 +11,35 @@ Require Import Logic.STLC.Replace.
 (* ELam: if a term evaluates to a value, abstracting preserves evaluation       *) 
 (* EAppN: evaluation for application, neutral case                              *)
 (* EAppL: evaluation for application, lambda case                               *)
-Inductive Eval (b v:Type)(e:Eq v) : Exp b v -> Exp b v -> Prop :=
-| EVar : forall (x:v), Eval b v e (Var x) (Var x)
-| EAnn : forall (t t':Exp b v) (Ty:T b),
-    Value t' -> Eval b v e t t' -> Eval b v e (Ann t Ty) t' 
-| ELam : forall (t t':Exp b v) (x:v),
-    Value t' -> Eval b v  e t t' -> Eval b v e (Lam x t) (Lam x t') 
-| EAppN : forall (t1 t1' t2 t2':Exp b v),
-    Neutral t1'         -> 
-    Value t2'           -> 
-    Eval b v e t1 t1'   -> 
-    Eval b v e t2 t2'   ->  
-    Eval b v e (App t1 t2) (App t1' t2')
-| EAppL : forall (t1 t1' t2 t2':Exp b v) (x:v),
-    Value t1'                               ->
-    Value t2'                               ->
-    Eval b v e t1 (Lam x t1')               ->
-    Eval b v e (subst (t2 // x) t1') t2'    ->
-    Eval b v e (App t1 t2) t2'
+Inductive Eval (b v:Type)(eq:Eq v) : Exp b v -> Exp b v -> Prop :=
+| EVar : forall (x:v), Eval b v eq (Var x) (Var x)
+| EAnn : forall (e e':Exp b v) (Ty:T b),
+    Value e' -> Eval b v eq e e' -> Eval b v eq (Ann e Ty) e' 
+| ELam : forall (e e':Exp b v) (x:v),
+    Value e' -> Eval b v eq e e' -> Eval b v eq (Lam x e) (Lam x e') 
+| EAppN : forall (e1 e1' e2 e2':Exp b v),
+    Neutral e1'         -> 
+    Value e2'           -> 
+    Eval b v eq e1 e1'  -> 
+    Eval b v eq e2 e2'  ->  
+    Eval b v eq (App e1 e2) (App e1' e2')
+| EAppL : forall (e1 e1' e2 e2':Exp b v) (x:v),
+    Value e1'                               ->
+    Value e2'                               ->
+    Eval b v eq e1 (Lam x e1')              ->
+    Eval b v eq (subst (e2 // x) e1') e2'   ->
+    Eval b v eq (App e1 e2) e2'
 .
 
-Arguments Eval  {b} {v} {e}.
-Arguments EVar  {b} {v} {e}.
-Arguments EAnn  {b} {v} {e}.
-Arguments ELam  {b} {v} {e}.
-Arguments EAppN {b} {v} {e}.
-Arguments EAppL {b} {v} {e}.
+Arguments Eval  {b} {v} {eq}.
+Arguments EVar  {b} {v} {eq}.
+Arguments EAnn  {b} {v} {eq}.
+Arguments ELam  {b} {v} {eq}.
+Arguments EAppN {b} {v} {eq}.
+Arguments EAppL {b} {v} {eq}.
 
 
-Notation "t >> t'" := (Eval t t')
+Notation "e >> e'" := (Eval e e')
     (at level 90, no associativity) : STLC_Eval_scope.
 
 Open Scope STLC_Eval_scope.
-
-
