coq/Logic/STLC/IsType.v
@@ -2,9 +2,9 @@ Require Import Logic.STLC.Syntax.
 Require Import Logic.STLC.Context.
 
 Inductive IsType (b v:Type) : @Context b v -> T b -> Prop :=
-| TVar : forall (G:Context) (Ty:b), 
-    G :> Ty -> 
-    IsType b v G (Base Ty)  
+| TVar : forall (G:Context) (t:b), 
+    G :> t -> 
+    IsType b v G (Base t)  
 | TFun : forall (G:Context) (Ty Ty':T b),
     IsType b v G Ty     -> 
     IsType b v G Ty'    -> 
@@ -27,19 +27,3 @@ Proof.
     - intros H3. subst. inversion H2.
     - assumption.
 Qed.
-
-(*
-Lemma IsTypeRev : forall (b v:Type) (G:@Context b v) (Ty:b) (Ty':T b),
-    (G ; Ty ::: * ) :- Ty' -> Ty' = (Base Ty) \/ G :- Ty'.
-Proof.
-    intros b v G Ty Ty' H1. remember (G ; Ty ::: * ) as G' eqn:E. 
-    revert G Ty E. induction H1 as [G Ty H2|G Ty Ty' H2 IH1 H3 IH2].
-    - intros G' Sy H4. subst. apply findTyRev' in H2. destruct H2 as [H2|H2].
-        + subst. left. reflexivity.
-        + right. constructor. assumption.
-    - intros G' Sy H4. right. constructor.
-      specialize IH1 with G' Sy. specialize IH2 with G' Sy.
-      destruct (IH1 H4) as [H5|H5]; destruct (IH2 H4) as [H6|H6].
-        + 
-Show.
-*)
